Bdd/Restrict.lean
@@ -1,72 +1,707 @@
 import Bdd.Basic
 import Bdd.Nary
+import Std.Data.HashMap.Lemmas
 
 namespace Restrict
 
+open RawBdd
+
 private structure State (n) (m) where
-  visited : Vector (Option (Pointer m)) m
-  newheap : Vector (Node n m) m
+  size : Nat
+  heap : Vector (RawNode n) size
+  cache : Std.HashMap (Pointer m) RawPointer
 
-private def lookup (j : Fin m) : StateM (State n m) (Option (Pointer m)) := fun ⟨V, M⟩ ↦ ⟨V[j], V, M⟩
-private def store (j : Fin m) (p : Pointer m) : StateM (State n m) (Pointer m) := fun ⟨V, M⟩ ↦ ⟨p, V.set j p, M⟩
-private def setj (j : Fin m) : Node n m → StateM (State n m) Unit := fun N ⟨V, M⟩ ↦ ⟨(), V, M.set j N⟩
+private def initial : State n m := ⟨_, (Vector.emptyWithCapacity 0), Std.HashMap.emptyWithCapacity 0⟩
 
-private def restrict_helper (O : OBdd n m) (b : Bool) (i : Fin n) :
-    StateM (State n m) (Pointer m) := do
-  let r := O.1.root
-  match hr : r with
-  | .terminal _ => return r
-  | .node j =>
-    match ← lookup j with
-    | some p => return p
-    | none =>
-      let N := O.1.heap[j]
-      if N.var > i
-      then -- Orderedness guarantees that we won't encounter i anywhere in this subgraph, so keep it as is.
-        store j r
-      else
-        if N.var < i
+private def Invariant (b : Bool) (i : Fin n) (O : OBdd n m) (s : State n m) :=
+  ∃ hh : (∀ i : Fin s.size, RawNode.Bounded i s.heap[i]),
+    ∀ (k : (Pointer m)) (p : RawPointer),
+      s.cache[k]? = some p →
+      (∀ j h, p = .inr j → (if (Pointer.toVar O.1.heap k) = i then (s.heap[j]'h).va.1 > (Pointer.toVar O.1.heap k) else (s.heap[j]'h).va.1 = (Pointer.toVar O.1.heap k))) ∧
+      ∃ hk1 : Bdd.Ordered ⟨O.1.heap, k⟩,
+          ∃ hp : p.Bounded s.size,
+            ∃ o : Bdd.Ordered ⟨cook_heap s.heap hh, p.cook hp⟩,
+                OBdd.evaluate ⟨⟨cook_heap s.heap hh, p.cook hp⟩, o⟩ = Nary.restrict (OBdd.evaluate ⟨⟨O.1.heap, k⟩, hk1⟩) b i
+
+private lemma inv_initial {b} {i} {O : OBdd n m} : Invariant b i O initial := by
+  constructor
+  · intro k p hp
+    simp only [initial, Std.HashMap.getElem?_emptyWithCapacity, reduceCtorEq] at hp
+  · rintro ⟨_, c⟩
+    simp only [initial, not_lt_zero'] at c
+
+private lemma heap_push_aux (s : State n m) (inv : Invariant b i O s)
+    (hNl : ∃ k : Pointer m, s.cache[k]? = some N.lo)
+    (hNh : ∃ k : Pointer m, s.cache[k]? = some N.hi)
+    (hNv : (if O.1.root.toVar O.1.heap = i then N.va.1 > (O.1.root.toVar O.1.heap).1 else N.va.1 = (O.1.root.toVar O.1.heap).1))
+    (hxl : ∀ j h (_ : N.lo = .inr j), N.va.1 < (s.heap[j]'h).va.1)
+    (hxh : ∀ j h (_ : N.hi = .inr j), N.va.1 < (s.heap[j]'h).va.1)
+    (hh : ∀ h0 (h1 : Bdd.Ordered _),
+      OBdd.evaluate ⟨⟨cook_heap (s.heap.push N) h0, .node ⟨s.size, by simp⟩⟩, h1⟩ = Nary.restrict (O.evaluate) b i) :
+    Invariant b i O
+      { size := s.size + 1, heap := s.heap.push N, cache := s.cache.insert (O.1.root) (Sum.inr s.size) } := by
+  rcases hNl with ⟨kl, hkl⟩
+  rcases hNh with ⟨kh, hkh⟩
+  have hN : RawNode.Bounded s.size N := by
+    simp only [RawNode.Bounded]
+    constructor
+    · exact (inv.2 kl N.lo hkl).2.2.1
+    · exact (inv.2 kh N.hi hkh).2.2.1
+  have : ∀ (i : Fin (s.size + 1)), RawNode.Bounded (↑i) (s.heap.push N)[i] := by
+    intro i
+    simp only [Fin.getElem_fin]
+    rw [Vector.getElem_push]
+    split
+    next hi => exact inv.1 ⟨i.1, hi⟩
+    next hi =>
+      have : i.1 = s.size := by omega
+      rw [this]
+      exact hN
+  use this
+  intro k p
+  simp only
+  intro hp
+  rw [Std.HashMap.getElem?_insert] at hp
+  simp only [beq_iff_eq, Vector.take_eq_extract] at hp
+  split at hp
+  next heq =>
+    subst heq
+    constructor
+    · intro j hs hj
+      rw [Vector.getElem_push]
+      split
+      next heqq =>
+        injection hp with hpp
+        rw [hj] at hpp
+        injection hpp with hppp
+        split
+        next contra => rw [hppp] at contra; absurd contra; simp only [lt_self_iff_false,
+          not_false_eq_true]
+        next =>
+          split at hNv
+          next contra => simp_all only [Fin.val_fin_lt, Fin.getElem_fin, lt_add_iff_pos_right,
+            Nat.lt_one_iff, pos_of_gt, Nat.succ_eq_add_one, Fin.coe_eq_castSucc, lt_self_iff_false,
+            not_false_eq_true, gt_iff_lt, Fin.castSucc_lt_castSucc_iff, Fin.coe_castSucc]
+          next contra => contradiction
+      next heqq =>
+        split
+        next contra => injection hp with hi; subst hi; injection hj with hi; rw [hi] at contra; absurd contra; simp only [lt_self_iff_false,
+          not_false_eq_true]
+        next =>
+          split at hNv
+          next => simp_all only [Fin.val_fin_lt, Fin.getElem_fin, Fin.natCast_eq_last,
+            Option.some.injEq, Nat.succ_eq_add_one, Fin.coe_eq_castSucc, not_true_eq_false]
+          next contra => rw [← hNv]
+    use O.2
+    injection hp with hpe
+    subst hpe
+    have hb : RawPointer.Bounded (s.size + 1) (Sum.inr s.size) := by intro i hi; injection hi with hie; subst hie; simp
+    use hb
+    have hoo : Bdd.Ordered ⟨cook_heap (s.heap.push N) this, RawPointer.cook (Sum.inr s.size) hb⟩ := by
+      apply Bdd.ordered_of_low_high_ordered rfl
+      · simp only [Bdd.low, cook_heap]
+        simp only [Fin.getElem_fin, Vector.getElem_ofFn, Vector.getElem_push_eq]
+        rw [← cook_low]
+        swap; apply RawPointer.bounded_of_le (inv.2 kl N.lo hkl).2.2.1; simp only [le_add_iff_nonneg_right, zero_le]
+        rcases (inv.2 kl N.lo hkl).2.2.2 with that
+        apply push_ordered
+        · exact this
+        · exact that.1
+      ·
+        simp [Nat.succ_eq_add_one, Bdd.var, gt_iff_lt, cook_heap, Bdd.low, RawPointer.cook]
+        cases heq : N.lo with
+        | inl val =>
+          rw [← cook_low]
+          simp_rw [heq]
+          simp only [RawPointer.cook, Pointer.toVar_terminal_eq, Nat.succ_eq_add_one,
+            Fin.natCast_eq_last, Fin.castSucc_lt_last]
+          apply RawPointer.bounded_of_le (inv.2 kl N.lo hkl).2.2.1; simp only [le_add_iff_nonneg_right, zero_le]
+        | inr val =>
+          have hvs : val < s.size := by
+            apply RawPointer.bounded_of_le (inv.2 kl N.lo hkl).2.2.1 .refl heq
+          rw [← cook_low]
+          simp_rw [heq]
+          simp only [RawNode.cook, RawPointer.cook, Pointer.toVar_node_eq, Nat.succ_eq_add_one,
+            Fin.getElem_fin, Vector.getElem_ofFn, Fin.coe_eq_castSucc, Fin.castSucc_lt_castSucc_iff]
+          rw [Vector.getElem_push_lt]
+          have hvs : val < s.size := by
+            apply RawPointer.bounded_of_le (inv.2 kl N.lo hkl).2.2.1 .refl heq
+          exact hxl _ hvs heq
+          exact hvs
+          apply RawPointer.bounded_of_le (inv.2 kl N.lo hkl).2.2.1; simp only [le_add_iff_nonneg_right, zero_le]
+      · simp only [Bdd.high, cook_heap]
+        simp only [Fin.getElem_fin, Vector.getElem_ofFn, Vector.getElem_push_eq]
+        rw [← cook_high]
+        swap; apply RawPointer.bounded_of_le (inv.2 kh N.hi hkh).2.2.1; simp only [le_add_iff_nonneg_right, zero_le]
+        rcases (inv.2 kh N.hi hkh).2.2.2 with that
+        apply push_ordered
+        · exact this
+        · exact that.1
+      ·
+        simp [Nat.succ_eq_add_one, Bdd.var, gt_iff_lt, cook_heap, Bdd.high, RawPointer.cook]
+        cases heq : N.hi with
+        | inl val =>
+          rw [← cook_high]
+          simp_rw [heq]
+          simp only [RawPointer.cook, Pointer.toVar_terminal_eq, Nat.succ_eq_add_one,
+            Fin.natCast_eq_last, Fin.castSucc_lt_last]
+          apply RawPointer.bounded_of_le (inv.2 kh N.hi hkh).2.2.1; simp only [le_add_iff_nonneg_right, zero_le]
+        | inr val =>
+          have hvs : val < s.size := by
+            apply RawPointer.bounded_of_le (inv.2 _ _ hkh).2.2.1 .refl heq
+          rw [← cook_high]
+          simp_rw [heq]
+          simp only [RawNode.cook, RawPointer.cook, Pointer.toVar_node_eq, Nat.succ_eq_add_one,
+            Fin.getElem_fin, Vector.getElem_ofFn, Fin.coe_eq_castSucc, Fin.castSucc_lt_castSucc_iff]
+          rw [Vector.getElem_push_lt]
+          exact hxh _ hvs heq
+          apply RawPointer.bounded_of_le (inv.2 kh N.hi hkh).2.2.1; simp only [le_add_iff_nonneg_right, zero_le]
+    use hoo
+    rw [show ⟨{ heap := O.1.heap, root := O.1.root }, _⟩ =  O by rfl]
+    simp [RawPointer.cook]
+    simp [RawPointer.cook] at hoo
+    have := hh _ (by exact hoo)
+    exact hh _ hoo
+  next heq =>
+    constructor
+    · intro j hs hj
+      rw [hj] at hp
+      rcases (inv.2 k _ hp) with ⟨inv1, inv2⟩
+      have := inv1 j (inv2.2.1 rfl) rfl
+      rw [Vector.getElem_push_lt (inv2.2.1 rfl)]
+      exact this
+    rcases (inv.2 k p hp) with that
+    use that.2.1
+    have hb : ∀ {i}, p = Sum.inr i → i < s.size + 1 :=
+      RawPointer.bounded_of_le that.2.2.1 (by simp only [le_add_iff_nonneg_right, zero_le])
+    use hb
+    have ho : Bdd.Ordered { heap := cook_heap (s.heap.push N) this, root := p.cook hb } := push_ordered that.2.2.2.1
+    use ho
+    ext I
+    calc _
+      _ = OBdd.evaluate ⟨{ heap := cook_heap (s.heap) inv.1, root := p.cook that.2.2.1 }, that.2.2.2.1⟩ I := by
+        rw [OBdd.evaluate_eq_evaluate_of_ordered_heap_all_reachable_eq]
+        · simp only [Fin.getElem_fin]
+          intro j hj
+          use (by omega)
+          simp [cook_heap]
+          exact RawNode.cook_equiv
+        · simp only [RawPointer.cook_equiv]
+    rw [that.2.2.2.2]
+
+private def heap_push (N : RawNode n) (s : (State n m)) (inv : Invariant b i O s)
+    (hNl : ∃ k : Pointer m, s.cache[k]? = some N.lo)
+    (hNh : ∃ k : Pointer m, s.cache[k]? = some N.hi)
+    (hNv : (if O.1.root.toVar O.1.heap = i then N.va.1 > (O.1.root.toVar O.1.heap).1 else N.va.1 = (O.1.root.toVar O.1.heap).1))
+    (hxl : ∀ j h (_ : N.lo = .inr j), N.va.1 < (s.heap[j]'h).va.1)
+    (hxh : ∀ j h (_ : N.hi = .inr j), N.va.1 < (s.heap[j]'h).va.1)
+    (hh : ∀ h0 (h1 : Bdd.Ordered _),
+      OBdd.evaluate ⟨⟨cook_heap (s.heap.push N) h0, .node ⟨s.size, by simp⟩⟩, h1⟩ = Nary.restrict (O.evaluate) b i)
+    (hc : s.cache[O.1.root]? = none) :
+    { r : State n m × RawPointer //
+      (Invariant b i O r.1) ∧
+      (r.1.cache[O.1.root]? = some r.2) ∧
+      s.size ≤ r.1.size ∧
+      (∀ (k : Pointer m),
+        (∀ p, s.cache[k]? = some p → r.1.cache[k]? = some p) ∧
+        (r.1.cache[k]? = none → s.cache[k]? = none) ∧
+        (s.cache[k]? = none → (∃ p, r.1.cache[k]? = some p) → Pointer.Reachable O.1.heap O.1.root k))
+    } :=
+  ⟨⟨⟨s.size + 1, s.heap.push N, s.cache.insert O.1.root (.inr s.size)⟩, .inr s.size⟩, by
+    simp only [Prod.exists]
+    constructor
+    · exact heap_push_aux s inv hNl hNh hNv hxl hxh hh
+    · constructor
+      · simp only [Std.HashMap.getElem?_insert_self]
+      · constructor
+        · simp only [le_add_iff_nonneg_right, zero_le]
+        · intro k
+          constructor
+          · intro p hkp
+            rw [← hkp]
+            simp only [Std.HashMap.getElem?_insert, beq_iff_eq, ite_eq_right_iff]
+            intro contra
+            rw [← contra] at hkp
+            rw [hkp] at hc
+            contradiction
+          · constructor
+            · simp only [getElem?_eq_none_iff, Std.HashMap.mem_insert, beq_iff_eq, not_or,
+                and_imp, imp_self, implies_true]
+            · rintro hk ⟨q, hq⟩
+              simp only [Std.HashMap.getElem?_insert, beq_iff_eq, ite_eq_right_iff] at hq
+              split at hq
+              next heqq => subst heqq; constructor
+              next heqq => rw [hk] at hq; contradiction
+  ⟩
+
+private lemma insert_terminal_invariant (s0 : State n m) (inv : Invariant b i O s0) (ho : O.1.root = .terminal b') :
+    Invariant b i O { size := s0.size, heap := s0.heap, cache := s0.cache.insert O.1.root (Sum.inl b') } := by
+  constructor
+  intro k p hp
+  simp only at hp
+  simp only
+  rw [Std.HashMap.getElem?_insert] at hp
+  simp only [beq_iff_eq] at hp
+  split at hp
+  next heq =>
+    rw [← heq]
+    constructor
+    · intro j hj hjp
+      subst hjp
+      injection hp with hpp
+      contradiction
+    use O.2
+    injection hp with hpe
+    subst hpe
+    use (fun contra ↦ by contradiction)
+    simp [RawPointer.cook, ho, Bdd.Ordered_of_terminal]
+  next =>
+    constructor
+    · exact (inv.2 _ _ hp).1
+    exact (inv.2 _ _ hp).2
+
+private def restrict_helper (O : OBdd n m) (b : Bool) (i : Fin n) (s0 : State n m) (inv : Invariant b i O s0) :
+    { r : State n m × RawPointer //
+      (Invariant b i O r.1) ∧
+      (r.1.cache[O.1.root]? = some r.2) ∧
+      (s0.size ≤ r.1.size) ∧
+      (∀ (k : Pointer m),
+        (∀ p, s0.cache[k]? = some p → r.1.cache[k]? = some p) ∧
+        (r.1.cache[k]? = none → s0.cache[k]? = none) ∧
+        (s0.cache[k]? = none → (∃ p, r.1.cache[k]? = some p) → Pointer.Reachable O.1.heap O.1.root k))
+    } :=
+  match hc : s0.cache[O.1.root]? with
+  | some root =>
+    ⟨ ⟨s0, root⟩, ⟨inv, hc, .refl,
+      by
+        intro k
+        constructor
+        · intro p h
+          exact h
+        · constructor
+          · intro h
+            exact h
+          · rintro h ⟨_, c⟩
+            rw [h] at c
+            contradiction,
+      ⟩
+    ⟩
+  | none =>
+    match O_root_def : O.1.root with
+    | .terminal b' =>
+        ⟨⟨⟨s0.size, s0.heap, s0.cache.insert O.1.root (.inl b')⟩, .inl b'⟩, by
+          simp only [Prod.exists]
+          constructor
+          · exact insert_terminal_invariant s0 inv O_root_def
+          · constructor
+            · simp only [O_root_def, Std.HashMap.getElem?_insert_self]
+            · constructor
+              · exact .refl
+              ·
+                intro k
+                constructor
+                · intro p hp
+                  rw [← hp]
+                  simp only [Std.HashMap.getElem?_insert, beq_iff_eq, ite_eq_right_iff]
+                  intro contra
+                  subst contra
+                  rw [hc] at hp
+                  contradiction
+                · constructor
+                  · simp only [getElem?_eq_none_iff, Std.HashMap.mem_insert, beq_iff_eq, not_or,
+                      and_imp, imp_self, implies_true]
+                  · rintro h1 ⟨p, hp⟩
+                    simp only [Std.HashMap.getElem?_insert,beq_iff_eq] at hp
+                    split at hp
+                    next heq =>
+                      subst heq
+                      simp only [O_root_def]
+                      constructor
+                    next heq => rw [h1] at hp; contradiction
+        ⟩
+    | .node j =>
+        if hlt : O.1.heap[j].var = i
         then
-          let l ← restrict_helper (O.low  hr) b i
-          let h ← restrict_helper (O.high hr) b i
-          setj j ⟨N.var, l, h⟩
-          store j r
-        else -- Found a node with variable i, short-circuit to the appropriate child.
-          store j (if b then N.high else N.low)
+          if hb : b
+          then
+            let ⟨⟨sl, rl⟩, ⟨invl, hl, hsl, hlp⟩⟩ := restrict_helper (O.high O_root_def) b i s0 inv
+            ⟨ ⟨⟨sl.size, sl.heap, sl.cache.insert O.1.root rl⟩, rl⟩,
+              by
+                constructor
+                · intro k p
+                  simp only
+                  intro hkp
+                  simp only [Std.HashMap.getElem?_insert,beq_iff_eq] at hkp
+                  split at hkp
+                  next heq =>
+                    subst heq
+                    injection hkp with hinj
+                    subst hinj
+                    constructor
+                    · intro j' hj1 hrj
+                      subst hrj
+                      have that : O.1.heap[j].var < (Pointer.toVar O.1.heap (O.high O_root_def).1.root) := by
+                        have := OBdd.var_lt_high_var (O := O) (h := O_root_def)
+                        simp only [OBdd.var, Nat.succ_eq_add_one, Bdd.var, OBdd.high_heap_eq_heap,
+                          Fin.val_fin_lt] at this
+                        rw [O_root_def] at this
+                        simp only [Pointer.toVar] at this
+                        exact this
+                      have := (invl.2 _ _ hl).1 _ hj1 rfl
+                      split at this
+                      next hsp =>
+                        rw [← hlt] at hsp
+                        rw [← hsp] at that
+                        absurd that
+                        simp only [Nat.succ_eq_add_one, OBdd.high_heap_eq_heap, lt_self_iff_false,
+                          not_false_eq_true]
+                      next hsp =>
+                        rw [← hlt]
+                        simp_all only [getElem?_eq_none_iff,
+                          Fin.getElem_fin, OBdd.low_heap_eq_heap, forall_exists_index,
+                          Nat.succ_eq_add_one, Fin.coe_eq_castSucc, Pointer.toVar_node_eq,
+                          Fin.coe_castSucc, gt_iff_lt, ite_true]
+                        exact that
+                    · use O.2
+                      have := (invl.2 _ _ hl).2.2
+                      use this.1
+                      use this.2.1
+                      rw [this.2.2]
+                      have triv {ho} : ⟨{ heap := O.1.heap, root := O.1.root }, ho⟩ = O := rfl
+                      rw [triv]
+                      have that := OBdd.evaluate_node'' O_root_def
+                      rw [that]
+                      rw [Nary.restrict_if]
+                      rw [hlt]
+                      simp only [OBdd.high_heap_eq_heap, hb, Fin.getElem_fin,
+                        Vector.getElem_set_self, ↓reduceIte]
+                      ext I
+                      conv =>
+                        rhs
+                        congr
+                        simp only [Nary.restrict, Vector.getElem_set_self]
+                      rfl
+                  next heq => exact (invl.2 _ _ hkp),
+              by simp only [O_root_def, Std.HashMap.getElem?_insert_self],
+              by exact hsl,
+              by
+                intro k
+                constructor
+                · intro p hkp
+                  simp only [Std.HashMap.getElem?_insert, beq_iff_eq]
+                  split
+                  next heq =>
+                    subst heq
+                    rw [hkp] at hc
+                    contradiction
+                  next => exact (hlp k).1 p hkp
+                · constructor
+                  · simp only [Std.HashMap.getElem?_insert, beq_iff_eq]
+                    split
+                    next heq =>
+                      subst heq
+                      simp only [reduceCtorEq, getElem?_eq_none_iff, IsEmpty.forall_iff]
+                    next => exact (hlp k).2.1
+                  · simp only [Std.HashMap.getElem?_insert, beq_iff_eq]
+                    split
+                    next heq =>
+                      subst heq
+                      rw [hc]
+                      simp only [Option.some.injEq, exists_eq', forall_const, O_root_def]
+                      left
+                    next =>
+                      intro hkn hhh
+                      rw [← O_root_def]
+                      trans (O.high O_root_def).1.root
+                      · exact OBdd.reachable_of_edge (Bdd.edge_of_high O.1 (h := O_root_def))
+                      · exact (hlp k).2.2 hkn hhh
+            ⟩
+          else
+            let ⟨⟨sl, rl⟩, ⟨invl, hl, hsl, hlp⟩⟩ := restrict_helper (O.low O_root_def) b i s0 inv
+            ⟨⟨⟨sl.size, sl.heap, sl.cache.insert O.1.root rl⟩, rl⟩,
+              by
+                constructor
+                · intro k p
+                  simp only
+                  intro hkp
+                  simp only [Std.HashMap.getElem?_insert,beq_iff_eq] at hkp
+                  split at hkp
+                  next heq =>
+                    subst heq
+                    injection hkp with hinj
+                    subst hinj
+                    constructor
+                    · intro j' hj1 hrj
+                      subst hrj
+                      have that : O.1.heap[j].var < (Pointer.toVar O.1.heap (O.low O_root_def).1.root) := by
+                        have := OBdd.var_lt_low_var (O := O) (h := O_root_def)
+                        simp only [OBdd.var, Nat.succ_eq_add_one, Bdd.var, OBdd.low_heap_eq_heap,
+                          Fin.val_fin_lt] at this
+                        rw [O_root_def] at this
+                        simp only [Pointer.toVar] at this
+                        exact this
+                      have := (invl.2 _ _ hl).1 _ hj1 rfl
+                      split at this
+                      next hsp =>
+                        rw [← hlt] at hsp
+                        rw [← hsp] at that
+                        absurd that
+                        simp only [Nat.succ_eq_add_one, OBdd.low_heap_eq_heap, lt_self_iff_false,
+                          not_false_eq_true]
+                      next hsp =>
+                        rw [← hlt]
+                        simp_all only [getElem?_eq_none_iff,
+                          Fin.getElem_fin, OBdd.low_heap_eq_heap, forall_exists_index,
+                          Nat.succ_eq_add_one, Fin.coe_eq_castSucc, Pointer.toVar_node_eq,
+                          Fin.coe_castSucc, gt_iff_lt, ite_true]
+                        exact that
+                    · use O.2
+                      have := (invl.2 _ _ hl).2.2
+                      use this.1
+                      use this.2.1
+                      rw [this.2.2]
+                      have triv {ho} : ⟨{ heap := O.1.heap, root := O.1.root }, ho⟩ = O := rfl
+                      rw [triv]
+                      have that := OBdd.evaluate_node'' O_root_def
+                      rw [that]
+                      rw [Nary.restrict_if]
+                      rw [hlt]
+                      simp only [OBdd.low_heap_eq_heap, hb, Fin.getElem_fin,
+                        Vector.getElem_set_self, ↓reduceIte]
+                      ext I
+                      conv =>
+                        rhs
+                        congr
+                        simp only [Nary.restrict, Vector.getElem_set_self]
+                      rfl
+                  next heq => exact (invl.2 _ _ hkp),
+              by simp only [O_root_def, Std.HashMap.getElem?_insert_self],
+              by exact hsl,
+              by
+                intro k
+                constructor
+                · intro p hkp
+                  simp only [Std.HashMap.getElem?_insert, beq_iff_eq]
+                  split
+                  next heq =>
+                    subst heq
+                    rw [hkp] at hc
+                    contradiction
+                  next => exact (hlp k).1 p hkp
+                · constructor
+                  · simp only [Std.HashMap.getElem?_insert, beq_iff_eq]
+                    split
+                    next heq =>
+                      subst heq
+                      simp only [reduceCtorEq, getElem?_eq_none_iff, IsEmpty.forall_iff]
+                    next => exact (hlp k).2.1
+                  · simp only [Std.HashMap.getElem?_insert, beq_iff_eq]
+                    split
+                    next heq =>
+                      subst heq
+                      rw [hc]
+                      simp only [Option.some.injEq, exists_eq', forall_const, O_root_def]
+                      left
+                    next =>
+                      intro hkn hhh
+                      rw [← O_root_def]
+                      trans (O.low O_root_def).1.root
+                      · exact OBdd.reachable_of_edge (Bdd.edge_of_low O.1 (h := O_root_def))
+                      · exact (hlp k).2.2 hkn hhh
+          ⟩
+        else
+          let ⟨⟨sl, rl⟩, ⟨invl, hl, hsl, hlp⟩⟩ := restrict_helper (O.low O_root_def) b i s0 inv
+          let ⟨⟨sh, rh⟩, ⟨invh, hh, hsh, hhp⟩⟩ := restrict_helper (O.high O_root_def) b i sl invl
+          let ⟨r, ⟨invv, hv, hsv, hvp⟩⟩ :=
+            heap_push (O := O)
+              ⟨⟨O.1.heap[j].var.1, by omega⟩, rl, rh⟩ sh invh
+              (by
+                use (O.low O_root_def).1.root
+                simp only
+                exact (hhp _).1 _ hl
+              )
+              ⟨_, hh⟩
+              (by
+                simp only
+                rw [O_root_def]
+                simp only [Fin.getElem_fin] at hlt
+                simp only [Nat.succ_eq_add_one, Pointer.toVar_node_eq, Fin.getElem_fin,
+                  Fin.coe_eq_castSucc, Fin.castSucc_inj, Fin.coe_castSucc, gt_iff_lt,
+                  lt_self_iff_false, if_false_left, and_true]
+                omega
+              )
+              (by
+                intro j' hj1
+                simp only [Fin.getElem_fin]
+                intro hj2
+                have := (hhp _).1 _ hl
+                simp only at this
+                rw [hj2] at this
+                have that := (invh.2 _ (.inr j') this).1 _ hj1 rfl
+                simp only at that
+                have hll : O.1.heap[j.1].var.1 < (Pointer.toVar O.1.heap (O.low O_root_def).1.root).1 := by
+                  have := OBdd.var_lt_low_var (O := O) (h := O_root_def)
+                  simp only [OBdd.var, Nat.succ_eq_add_one, Bdd.var, OBdd.low_heap_eq_heap,
+                    Fin.val_fin_lt] at this
+                  rw [O_root_def] at this
+                  nth_rw 1 [Pointer.toVar] at this
+                  rw [Fin.lt_iff_val_lt_val, Fin.getElem_fin] at this
+                  convert this using 1
+                  simp only [Nat.succ_eq_add_one, Fin.coe_eq_castSucc, Fin.coe_castSucc]
+                split at that
+                next =>
+                  trans (Pointer.toVar O.1.heap (O.low O_root_def).1.root).1
+                  · exact hll
+                  · exact that
+                next =>
+                  rw [that]
+                  exact hll
+              )
+              (by
+                intro j' hj1
+                simp only [Fin.getElem_fin]
+                intro hj2
+                have that := (invh.2 _ _ hh).1 _ hj1 hj2
+                have hll : O.1.heap[j.1].var.1 < (Pointer.toVar O.1.heap (O.high O_root_def).1.root).1 := by
+                  have := OBdd.var_lt_high_var (O := O) (h := O_root_def)
+                  simp only [OBdd.var, Nat.succ_eq_add_one, Bdd.var, OBdd.high_heap_eq_heap,
+                    Fin.val_fin_lt] at this
+                  rw [O_root_def] at this
+                  nth_rw 1 [Pointer.toVar] at this
+                  rw [Fin.lt_iff_val_lt_val, Fin.getElem_fin] at this
+                  convert this using 1
+                  simp only [Nat.succ_eq_add_one, Fin.coe_eq_castSucc, Fin.coe_castSucc]
+                split at that
+                next =>
+                  trans (Pointer.toVar O.1.heap (O.high O_root_def).1.root).1
+                  · exact hll
+                  · exact that
+                next =>
+                  rw [that]
+                  exact hll
+              )
+              (by
+                intro h0 h1
+                symm
+                rw [OBdd.evaluate_node'' O_root_def]
+                rw [Nary.restrict_if]
+                conv =>
+                  rhs
+                  rw [OBdd.evaluate_node']
+                simp only [Fin.getElem_fin, Fin.eta]
+                ext I
+                congr 1
+                · simp only [Nary.restrict, cook_heap, RawNode.cook, Fin.getElem_fin,
+                  Vector.getElem_ofFn, Vector.getElem_push_eq, eq_iff_iff, Bool.coe_iff_coe]
+                  exact Vector.getElem_set_ne _ _ (fun contra ↦ by simp only [Fin.val_eq_val] at contra; rw [contra] at hlt; contradiction)
+                · have := (invh.2 (O.high O_root_def).1.root rh hh).2
+                  conv =>
+                    rhs
+                    congr
+                    congr
+                    congr
+                    rfl
+                    simp [cook_heap, RawNode.cook]
+                    rfl
+                    rfl
+                  symm
+                  calc _
+                    _ = OBdd.evaluate ⟨⟨cook_heap sh.heap _, rh.cook _⟩, _⟩ I := by
+                      rw [push_evaluate]
+                      · exact this.2.1
+                      · exact push_ordered this.2.2.1
+                      · exact this.2.2.1
+                    _ = _ := by
+                      have := this.2.2.2
+                      simp only [Vector.take_eq_extract, OBdd.high_heap_eq_heap] at this
+                      rw [this]
+                      rfl
+                · conv =>
+                    rhs
+                    congr
+                    congr
+                    congr
+                    rfl
+                    simp [cook_heap, RawNode.cook]
+                    rfl
+                    rfl
+                  symm
+                  have : sh.cache[(O.low O_root_def).1.root]? = some rl := by
+                    apply (hhp _).1
+                    exact hl
+                  have := invh.2 (O.low O_root_def).1.root rl this
+                  calc _
+                    _ = OBdd.evaluate ⟨⟨cook_heap sh.heap _, rl.cook _⟩, _⟩ I := by
+                      rw [push_evaluate]
+                      · exact this.2.2.1
+                      · exact push_ordered this.2.2.2.1
+                      · exact this.2.2.2.1
+                    _ = _ := by
+                      have := this.2.2.2.2
+                      simp only [Vector.take_eq_extract, OBdd.high_heap_eq_heap] at this
+                      rw [this]
+                      rfl
+              )
+              (by
+                cases heq : sh.cache[O.1.root]? with
+                | none => rfl
+                | some val =>
+                  cases heqq : sl.cache[O.1.root]? with
+                  | none =>
+                    have := ((hhp _).2.2 heqq ⟨val, heq⟩)
+                    simp only [OBdd.high_heap_eq_heap] at this
+                    absurd this
+                    apply OBdd.not_oedge_reachable
+                    exact oedge_of_high
+                  | some val =>
+                    have := ((hlp _).2.2 hc ⟨_, heqq⟩)
+                    simp only [OBdd.low_heap_eq_heap] at this
+                    absurd this
+                    apply OBdd.not_oedge_reachable
+                    exact oedge_of_low
+              )
+          ⟨ r,
+            invv,
+            (by rw [O_root_def] at hv; exact hv),
+            .trans hsl (.trans hsh hsv),
+            by
+              intro k
+              constructor
+              · intro p hp
+                apply (hvp _).1
+                apply (hhp _).1
+                apply (hlp _).1
+                exact hp
+              · constructor
+                · intro hk
+                  apply (hlp _).2.1
+                  apply (hhp _).2.1
+                  apply (hvp _).2.1
+                  exact hk
+                · intro hk hkp
+                  rw [← O_root_def]
+                  cases heq : sh.cache[k]? with
+                  | none =>
+                    apply (hvp _).2.2 heq hkp
+                  | some w =>
+                    cases heqq : sl.cache[k]? with
+                    | none =>
+                      have := (hhp _).2.2 heqq ⟨_, heq⟩
+                      · trans (O.high O_root_def).1.root
+                        · apply OBdd.reachable_of_edge
+                          exact oedge_of_high.2
+                        · exact this
+                    | some ww =>
+                      have := (hlp _).2.2 hk ⟨_, heqq⟩
+                      · trans (O.low O_root_def).1.root
+                        · apply OBdd.reachable_of_edge
+                          exact oedge_of_low.2
+                        · exact this
+          ⟩
 termination_by O
 
-private def restrict (O : OBdd n m) (b : Bool) (i : Fin n) : Bdd n m :=
-  let ⟨r, _, M⟩ := restrict_helper O b i ⟨Vector.replicate m none, O.1.heap⟩
-  ⟨M,r⟩
-
-@[simp]
-private lemma restrict_toVar : Pointer.toVar (restrict O b i).heap p = Pointer.toVar O.1.heap p := by
-  sorry
-
-private lemma restrict_edge_trans : Edge (restrict O b i).heap p q → Relation.TransGen (Edge O.1.heap) p q := by
-  sorry
-
-private lemma restrict_reachable : Pointer.Reachable (restrict O b i).heap (restrict O b i).root p → Pointer.Reachable O.1.heap O.1.root p := by
-  intro h
-  induction h with
-  | refl =>
-    simp only [restrict]
-    split
-    next M heq => sorry
-  | tail r e ih =>
-    exact .trans ih (Relation.TransGen.to_reflTransGen (restrict_edge_trans e))
-
-private lemma restrict_ordered : Bdd.Ordered (restrict O b i) := by
-  rintro ⟨x, hx⟩ ⟨y, hy⟩ hxy
-  simp_all only [Bdd.RelevantEdge, Bdd.RelevantMayPrecede, Pointer.MayPrecede, Nat.succ_eq_add_one]
-  have : Pointer.Reachable O.1.heap O.1.root x := restrict_reachable hx
-  rw [restrict_toVar]
-  rw [restrict_toVar]
-  exact Pointer.toVar_lt_of_trans_edge_of_ordered (Bdd.ordered_of_reachable this) (restrict_edge_trans hxy)
-
-def orestrict (O : OBdd n m) (b : Bool) (i : Fin n) : OBdd n m := ⟨restrict O b i, restrict_ordered⟩
-
-@[simp]
-lemma orestrict_evaluate {O : OBdd n m} : (orestrict O b i).evaluate = Nary.restrict (O.evaluate) b i := sorry
+def orestrict (O : OBdd n m) (b : Bool) (i : Fin n) : (s : Nat) × { W : OBdd n s // W.evaluate = Nary.restrict O.evaluate b i } :=
+  let ⟨⟨⟨siz, heap, _⟩, root⟩, h1, h2⟩:= restrict_helper O b i initial inv_initial
+  ⟨ siz, ⟨⟨cook_heap heap h1.1, root.cook (h1.2 _ root h2.1).2.2.1⟩, (h1.2 _ root h2.1).2.2.2.1⟩, (h1.2 _ root h2.1).2.2.2.2 ⟩
 
 end Restrict
